{
 "cells": [
  {
   "cell_type": "markdown",
   "metadata": {},
   "source": [
    "# School Method for Solving Systems of Linear Equations"
   ]
  },
  {
   "cell_type": "code",
   "execution_count": 1,
   "metadata": {},
   "outputs": [],
   "source": [
    "import sympy as sp\n",
    "from sympy import symbols, Eq, expand, solve\n",
    "\n",
    "class EnhancedEq(Eq):\n",
    "    def __add__(self, other):\n",
    "        return EnhancedEq(self.lhs + other.lhs, self.rhs + other.rhs)\n",
    "\n",
    "    def __sub__(self, other):\n",
    "        return EnhancedEq(self.lhs - other.lhs, self.rhs - other.rhs)\n",
    "\n",
    "    def __mul__(self, scalar):\n",
    "        return EnhancedEq(scalar * self.lhs, scalar * self.rhs)\n",
    "\n",
    "    def __rmul__(self, scalar):\n",
    "        return self.__mul__(scalar)\n",
    "\n",
    "    def simplify(self):\n",
    "        return EnhancedEq(expand(self.lhs), expand(self.rhs))\n",
    "\n",
    "    def substitute(self, *args, **kwargs):\n",
    "        return EnhancedEq(self.lhs.subs(*args, **kwargs), self.rhs.subs(*args, **kwargs))\n",
    "\n",
    "    def solve_for(self, symbol):\n",
    "        return solve(self, symbol)\n",
    "\n",
    "# Example usage:\n",
    "x, y = symbols('x y')\n",
    "\n",
    "# Define equations\n",
    "eq1 = EnhancedEq(2*x + y, 5)\n",
    "eq2 = EnhancedEq(x - y, 1)"
   ]
  },
  {
   "cell_type": "code",
   "execution_count": 2,
   "metadata": {},
   "outputs": [
    {
     "name": "stdout",
     "output_type": "stream",
     "text": [
      "First equation:\n"
     ]
    },
    {
     "data": {
      "text/latex": [
       "$\\displaystyle 2 x + y = 5$"
      ],
      "text/plain": [
       "Eq(2*x + y, 5)"
      ]
     },
     "execution_count": 2,
     "metadata": {},
     "output_type": "execute_result"
    }
   ],
   "source": [
    "print(\"First equation:\")\n",
    "eq1"
   ]
  },
  {
   "cell_type": "code",
   "execution_count": 3,
   "metadata": {},
   "outputs": [
    {
     "name": "stdout",
     "output_type": "stream",
     "text": [
      "Second equation:\n"
     ]
    },
    {
     "data": {
      "text/latex": [
       "$\\displaystyle x - y = 1$"
      ],
      "text/plain": [
       "Eq(x - y, 1)"
      ]
     },
     "execution_count": 3,
     "metadata": {},
     "output_type": "execute_result"
    }
   ],
   "source": [
    "print(\"Second equation:\")\n",
    "eq2"
   ]
  },
  {
   "cell_type": "code",
   "execution_count": 4,
   "metadata": {},
   "outputs": [
    {
     "data": {
      "text/latex": [
       "$\\displaystyle 3 x = 6$"
      ],
      "text/plain": [
       "Eq(3*x, 6)"
      ]
     },
     "execution_count": 4,
     "metadata": {},
     "output_type": "execute_result"
    }
   ],
   "source": [
    "# Add the equations\n",
    "eq3 = eq1 + eq2\n",
    "eq3"
   ]
  },
  {
   "cell_type": "code",
   "execution_count": 5,
   "metadata": {},
   "outputs": [
    {
     "data": {
      "text/latex": [
       "$\\displaystyle 2$"
      ],
      "text/plain": [
       "2"
      ]
     },
     "execution_count": 5,
     "metadata": {},
     "output_type": "execute_result"
    }
   ],
   "source": [
    "# We have an equation with one unknown, so we can solve it\n",
    "sol_x = eq3.solve_for(x)[0]\n",
    "sol_x"
   ]
  },
  {
   "cell_type": "code",
   "execution_count": 6,
   "metadata": {},
   "outputs": [
    {
     "data": {
      "text/latex": [
       "$\\displaystyle 2 - y = 1$"
      ],
      "text/plain": [
       "Eq(2 - y, 1)"
      ]
     },
     "execution_count": 6,
     "metadata": {},
     "output_type": "execute_result"
    }
   ],
   "source": [
    "# Substitute the solution into equation 2\n",
    "eq2 = eq2.substitute(x, sol_x)\n",
    "eq2"
   ]
  },
  {
   "cell_type": "code",
   "execution_count": 7,
   "metadata": {},
   "outputs": [
    {
     "data": {
      "text/latex": [
       "$\\displaystyle 1$"
      ],
      "text/plain": [
       "1"
      ]
     },
     "execution_count": 7,
     "metadata": {},
     "output_type": "execute_result"
    }
   ],
   "source": [
    "# We get an equation with one unknown, so we can solve it\n",
    "eq2.solve_for(y)[0]"
   ]
  },
  {
   "cell_type": "code",
   "execution_count": 8,
   "metadata": {},
   "outputs": [
    {
     "data": {
      "text/plain": [
       "{x: 2, y: 1}"
      ]
     },
     "execution_count": 8,
     "metadata": {},
     "output_type": "execute_result"
    }
   ],
   "source": [
    "# Thus x=2, y=1\n",
    "# Verify with sympy\n",
    "sp.solve([eq1, eq2])"
   ]
  },
  {
   "cell_type": "markdown",
   "metadata": {},
   "source": [
    "---\n",
    "\n",
    "### Exercises for Students\n",
    "\n",
    "Solve the following systems of equations similarly to the example above:\n",
    "\n",
    "* $3x-2y=5, \\quad 2x+3y=7$,\n",
    "* $2x-3y=10, \\quad 4x+5y=20$,\n",
    "* $2x - y + z = 3, \\quad x + 2y - z = 1, \\quad 3x - y + 2z = 11$.\n",
    "* $2x-3y+4z+2t=2, \\quad 3x+2y-5z+3t=3, \\quad 4x-3y+2z-5t=4, \\quad 5x+4y-3z+2t=5$."
   ]
  },
  {
   "cell_type": "markdown",
   "metadata": {},
   "source": [
    "<h2><b>7. Linear Equations old school</b></h2>\n",
    "<hr/>\n",
    "\n",
    "<h4><B>Solution to System 1 </b></h4>\n",
    "\n",
    "$$\n",
    "\\begin{cases}\n",
    "3x - 2y = 5 \\\\\n",
    "2x + 3y = 7\n",
    "\\end{cases}\n",
    "$$\n",
    "\n",
    "**Step 1. Eliminate one variable (e.g.\\y).**\n",
    "\n",
    "Multiply the first equation by 3 and the second by 2:\n",
    "\n",
    "$$\n",
    "\\begin{aligned}\n",
    "(3x - 2y) \\cdot 3 &: 9x - 6y = 15 \\\\\n",
    "(2x + 3y) \\cdot 2 &: 4x + 6y = 14\n",
    "\\end{aligned}\n",
    "$$\n",
    "\n",
    "Add them to eliminate y:\n",
    "\n",
    "$$\n",
    "9x - 6y + 4x + 6y = 15 + 14 \\implies 13x = 29 \\implies x = \\frac{29}{13}\n",
    "$$\n",
    "\n",
    "**Step 2. Substitute** $$x = \\frac{29}{13}$$ back into one of the original equations (say $$3x - 2y = 5$$):\n",
    "\n",
    "$$\n",
    "3\\left(\\frac{29}{13}\\right) - 2y = 5\n",
    "$$\n",
    "\n",
    "$$\n",
    "\\frac{87}{13} - 2y = 5 \\implies -2y = 5 - \\frac{87}{13}\n",
    "$$\n",
    "\n",
    "$$\n",
    "5 = \\frac{65}{13}, \\text{ so } 5 - \\frac{87}{13} = \\frac{65}{13} - \\frac{87}{13} = -\\frac{22}{13}\n",
    "$$\n",
    "\n",
    "$$\n",
    "-2y = -\\frac{22}{13} \\implies y = \\frac{11}{13}\n",
    "$$\n",
    "\n",
    "Hence,\n",
    "\n",
    "$$\n",
    "(x,y) = \\left(\\frac{29}{13}, \\frac{11}{13}\\right)\n",
    "$$\n",
    "\n",
    "<h4><B>Solution to System 2 </b></h4>\n",
    "\n",
    "$$\n",
    "\\begin{cases}\n",
    "2x - 3y = 10 \\\\\n",
    "4x + 5y = 20\n",
    "\\end{cases}\n",
    "$$\n",
    "\n",
    "**Step 1. Eliminate one variable (e.g.\\y).**\n",
    "\n",
    "Multiply the first equation by 5 and the second by 3:\n",
    "\n",
    "$$\n",
    "\\begin{aligned}\n",
    "(2x - 3y) \\cdot 5 &: 10x - 15y = 50 \\\\\n",
    "(4x + 5y) \\cdot 3 &: 12x + 15y = 60\n",
    "\\end{aligned}\n",
    "$$\n",
    "\n",
    "Add them to eliminate y:\n",
    "\n",
    "$$\n",
    "10x - 15y + 12x + 15y = 50 + 60 \\implies 22x = 110 \\implies x = 5\n",
    "$$\n",
    "\n",
    "**Step 2. Substitute** $$x = 5$$ back into one of the original equations (say $$2x - 3y = 10$$):\n",
    "\n",
    "$$\n",
    "2 \\cdot 5 - 3y = 10 \\implies 10 - 3y = 10 \\implies -3y = 0 \\implies y = 0\n",
    "$$\n",
    "\n",
    "Hence,\n",
    "\n",
    "$$\n",
    "(x,y) = (5, 0)\n",
    "$$\n",
    "\n",
    "<h4><b>Solution to System 3 </b></h4>\n",
    "\n",
    "$$\n",
    "\\begin{cases}\n",
    "2x - y + z = 3 \\\\\n",
    "x + 2y - z = 1 \\\\\n",
    "3x - y + 2z = 11\n",
    "\\end{cases}\n",
    "$$\n",
    "\n",
    "Label these as:\n",
    "\n",
    "$$\n",
    "\\begin{aligned}\n",
    "(1) &: 2x - y + z = 3 \\\\\n",
    "(2) &: x + 2y - z = 1 \\\\\n",
    "(3) &: 3x - y + 2z = 11\n",
    "\\end{aligned}\n",
    "$$\n",
    "\n",
    "**Step 1. Add (1) and (2) to eliminate z:**\n",
    "\n",
    "$$\n",
    "(2x - y + z) + (x + 2y - z) = 3 + 1 \\implies 3x + y = 4\n",
    "$$\n",
    "\n",
    "Call this new equation:\n",
    "\n",
    "$$\n",
    "(4): 3x + y = 4\n",
    "$$\n",
    "\n",
    "**Step 2. Eliminate z between (1) and (3). For instance, double (1) and subtract (3):**\n",
    "\n",
    "$$\n",
    "(1) \\times 2: 4x - 2y + 2z = 6\n",
    "$$\n",
    "\n",
    "Subtract (3):\n",
    "\n",
    "$$\n",
    "(4x - 2y + 2z) - (3x - y + 2z) = 6 - 11\n",
    "$$\n",
    "\n",
    "On the left:\n",
    "\n",
    "$$\n",
    "4x - 3x = x, \\quad -2y - (-y) = -2y + y = -y, \\quad 2z - 2z = 0\n",
    "$$\n",
    "\n",
    "so\n",
    "\n",
    "$$\n",
    "x - y = -5\n",
    "$$\n",
    "\n",
    "Call this\n",
    "\n",
    "$$\n",
    "(5): x - y = -5\n",
    "$$\n",
    "\n",
    "**Step 3. Solve the 2x2 system given by (4) and (5):**\n",
    "\n",
    "$$\n",
    "\\begin{cases}\n",
    "3x + y = 4 \\\\\n",
    "x - y = -5\n",
    "\\end{cases}\n",
    "$$\n",
    "\n",
    "Add them to eliminate y:\n",
    "\n",
    "$$\n",
    "(3x + y) + (x - y) = 4 + (-5) \\implies 4x = -1 \\implies x = -\\frac{1}{4}\n",
    "$$\n",
    "\n",
    "Then substitute $$x = -\\frac{1}{4}$$ into (4) (or (5)):\n",
    "\n",
    "$$\n",
    "3\\left(-\\frac{1}{4}\\right) + y = 4 \\implies -\\frac{3}{4} + y = 4 \\implies y = 4 + \\frac{3}{4} = \\frac{16}{4} + \\frac{3}{4} = \\frac{19}{4}\n",
    "$$\n",
    "\n",
    "**Step 4. Find z using any of the original equations, say (1):**\n",
    "\n",
    "$$\n",
    "2x - y + z = 3\n",
    "$$\n",
    "\n",
    "Substitute $$x = -\\frac{1}{4}$$ and $$y = \\frac{19}{4}$$:\n",
    "\n",
    "$$\n",
    "2\\left(-\\frac{1}{4}\\right) - \\frac{19}{4} + z = 3\n",
    "$$\n",
    "\n",
    "$$\n",
    "-\\frac{1}{2} - \\frac{19}{4} + z = 3\n",
    "$$\n",
    "\n",
    "Convert everything to fourths:\n",
    "\n",
    "$$\n",
    "-\\frac{1}{2} = -\\frac{2}{4}, \\quad -\\frac{2}{4} - \\frac{19}{4} = -\\frac{21}{4}\n",
    "$$\n",
    "\n",
    "So;\n",
    "\n",
    "$$\n",
    "-\\frac{21}{4} + z = 3 \\implies z = 3 + \\frac{21}{4} = \\frac{12}{4} + \\frac{21}{4} = \\frac{33}{4}\n",
    "$$\n",
    "\n",
    "Hence,\n",
    "\n",
    "$$\n",
    "(x,y,z) = \\left(-\\frac{1}{4}, \\frac{19}{4}, \\frac{33}{4}\\right)\n",
    "$$\n",
    "\n",
    "<h4><b>Solution to System 4 </b></h4>\n",
    "\n",
    "$$\n",
    "\\begin{cases}\n",
    "2x - 3y + 4z + 2t = 2 \\\\\n",
    "3x + 2y - 5z + 3t = 3 \\\\\n",
    "4x - 3y + 2z - 5t = 4 \\\\\n",
    "5x + 4y - 3z + 2t = 5\n",
    "\\end{cases}\n",
    "$$\n",
    "\n",
    "Label them:\n",
    "\n",
    "$$\n",
    "\\begin{aligned}\n",
    "(\\mathrm{I}) &: 2x - 3y + 4z + 2t = 2 \\\\\n",
    "(\\mathrm{II}) &: 3x + 2y - 5z + 3t = 3 \\\\\n",
    "(\\mathrm{III}) &: 4x - 3y + 2z - 5t = 4 \\\\\n",
    "(\\mathrm{IV}) &: 5x + 4y - 3z + 2t = 5\n",
    "\\end{aligned}\n",
    "$$\n",
    "\n",
    "1. Combine (I) and (II) to eliminate x.\n",
    "\n",
    "Multiply (I) by 3:\n",
    "\n",
    "$$\n",
    "6x - 9y + 12z + 6t = 6\n",
    "$$\n",
    "\n",
    "Multiply (II) by 2:\n",
    "\n",
    "$$\n",
    "6x + 4y - 10z + 6t = 6\n",
    "$$\n",
    "\n",
    "Subtract one from the other:\n",
    "\n",
    "$$\n",
    "(6x - 9y + 12z + 6t) - (6x + 4y - 10z + 6t) = 6 - 6\n",
    "$$\n",
    "\n",
    "Left side:\n",
    "\n",
    "$$\n",
    "6x - 6x = 0, \\quad -9y - 4y = -13y, \\quad 12z - (-10z) = 12z + 10z = 22z, \\quad 6t - 6t = 0\n",
    "$$\n",
    "\n",
    "Right side: 0.\n",
    "\n",
    "Hence,\n",
    "\n",
    "$$\n",
    "-13y + 22z = 0 \\implies 13y = 22z \\implies y = \\frac{22}{13}z \\tag{A}\n",
    "$$\n",
    "\n",
    "2. Combine (I) and (III) to eliminate x.\n",
    "\n",
    "Multiply (I) by 4:\n",
    "\n",
    "$$\n",
    "8x - 12y + 16z + 8t = 8\n",
    "$$\n",
    "\n",
    "Multiply (III) by 2:\n",
    "\n",
    "$$\n",
    "8x - 6y + 4z - 10t = 8\n",
    "$$\n",
    "\n",
    "Subtract one from the other:\n",
    "\n",
    "$$\n",
    "(8x - 12y + 16z + 8t) - (8x - 6y + 4z - 10t) = 8 - 8\n",
    "$$\n",
    "\n",
    "Left side:\n",
    "\n",
    "$$\n",
    "8x - 8x = 0, \\quad -12y - (-6y) = -12y + 6y = -6y, \\quad 16z - 4z = 12z, \\quad 8t - (-10t) = 8t + 10t = 18t\n",
    "$$\n",
    "\n",
    "Right side: 0.\n",
    "\n",
    "Hence\n",
    "\n",
    "$$\n",
    "-6y + 12z + 18t = 0\n",
    "$$\n",
    "\n",
    "Divide by 6:\n",
    "\n",
    "$$\n",
    "-y + 2z + 3t = 0 \\implies y = 2z + 3t \\tag{B}\n",
    "$$\n",
    "\n",
    "3. Combine (A) and (B) to relate z and t.\n",
    "\n",
    "From (A):\n",
    "\n",
    "$$\n",
    "y = \\frac{22}{13}z\n",
    "$$\n",
    "\n",
    "From (B):\n",
    "\n",
    "$$\n",
    "y = 2z + 3t\n",
    "$$\n",
    "\n",
    "Set them equal:\n",
    "\n",
    "$$\n",
    "2z + 3t = \\frac{22}{13}z \\implies 3t = \\frac{22}{13}z - 2z\n",
    "$$\n",
    "\n",
    "$$\n",
    "2z = \\frac{26}{13}z, \\quad \\frac{22}{13}z - \\frac{26}{13}z = -\\frac{4}{13}z\n",
    "$$\n",
    "\n",
    "so\n",
    "\n",
    "$$\n",
    "3t = -\\frac{4}{13}z \\implies t = -\\frac{4}{39}z\n",
    "$$\n",
    "\n",
    "Hence from (A) or (B):\n",
    "\n",
    "$$\n",
    "y = 2z + 3\\left(-\\frac{4}{39}z\\right) = 2z - \\frac{12}{39}z = 2z - \\frac{4}{13}z\n",
    "$$\n",
    "\n",
    "4. Solve for x in terms of z.\n",
    "\n",
    "Use (I) again:\n",
    "\n",
    "$$\n",
    "2x - 3y + 4z + 2t = 2\n",
    "$$\n",
    "\n",
    "Substitute $$y = \\frac{22}{13}z$$ and $$t = -\\frac{4}{39}z$$:\n",
    "\n",
    "$$\n",
    "2x - 3\\left(\\frac{22}{13}z\\right) + 4z + 2\\left(-\\frac{4}{39}z\\right) = 2\n",
    "$$\n",
    "\n",
    "Compute step by step:\n",
    "\n",
    "$$\n",
    "-3 \\cdot \\frac{22}{13}z = -\\frac{66}{13}z, \\quad 4z = \\frac{52}{13}z\n",
    "$$\n",
    "\n",
    "Thus\n",
    "\n",
    "$$\n",
    "-\\frac{66}{13}z + \\frac{52}{13}z = -\\frac{14}{13}z\n",
    "$$\n",
    "\n",
    "$$\n",
    "2\\left(-\\frac{4}{39}z\\right) = -\\frac{8}{39}z\n",
    "$$\n",
    "\n",
    "Convert $$-\\frac{14}{13}z$$ to denominator 39:\n",
    "\n",
    "$$\n",
    "-\\frac{14}{13}z = -\\frac{14 \\times 3}{13 \\times 3}z = -\\frac{42}{39}z\n",
    "$$\n",
    "\n",
    "So\n",
    "\n",
    "$$\n",
    "-\\frac{42}{39}z - \\frac{8}{39}z = -\\frac{50}{39}z\n",
    "$$\n",
    "\n",
    "Thus the equation becomes:\n",
    "\n",
    "$$\n",
    "2x - \\frac{50}{39}z = 2 \\implies 2x = 2 + \\frac{50}{39}z \\implies x = 1 + \\frac{25}{39}z\n",
    "$$\n",
    "\n",
    "5. Use a remaining equation (e.g. (IV)) to pin down z.\n",
    "\n",
    "Equation (IV) is:\n",
    "\n",
    "$$\n",
    "5x + 4y - 3z + 2t = 5\n",
    "$$\n",
    "\n",
    "Substitute\n",
    "\n",
    "$$\n",
    "x = 1 + \\frac{25}{39}z, \\quad y = \\frac{22}{13}z, \\quad t = -\\frac{4}{39}z\n",
    "$$\n",
    "\n",
    "After computation and simplification you get:\n",
    "\n",
    "$$\n",
    "5 + \\frac{264}{39}z=5\n",
    "$$\n",
    "\n",
    "$$\n",
    "\\frac{264}{39}z = 0 \\implies z = 0\n",
    "$$\n",
    "\n",
    "6. Back-substitute z = 0.\n",
    "\n",
    "From z = 0,\n",
    "\n",
    "$$\n",
    "t = -\\frac{4}{39} \\cdot 0 = 0\n",
    "$$\n",
    "\n",
    "From\n",
    "\n",
    "$$\n",
    "y = \\frac{22}{13} \\cdot 0 = 0\n",
    "$$\n",
    "\n",
    "From\n",
    "\n",
    "$$\n",
    "x = 1 + \\frac{25}{39} \\cdot 0 = 1\n",
    "$$\n",
    "\n",
    "Hence,\n",
    "\n",
    "$$\n",
    "(x,y,z,t) = (1, 0, 0, 0)\n",
    "$$"
   ]
  }
 ],
 "metadata": {
  "kernelspec": {
   "display_name": "Python 3",
   "language": "python",
   "name": "python3"
  },
  "language_info": {
   "codemirror_mode": {
    "name": "ipython",
    "version": 3
   },
   "file_extension": ".py",
   "mimetype": "text/x-python",
   "name": "python",
   "nbconvert_exporter": "python",
   "pygments_lexer": "ipython3",
   "version": "3.11.9"
  }
 },
 "nbformat": 4,
 "nbformat_minor": 4
}
