{
 "cells": [
  {
   "cell_type": "markdown",
   "metadata": {},
   "source": [
    "## 18. Functions\n",
    "\n",
    "1. Draw in a single Geogebra notebook the following functions:\n",
    "   - $f(x) = x^2$\n",
    "   - $g(x) = \\sqrt{x}$\n",
    "   - $h(x) = \\frac{1}{x}$\n",
    "   - $j(x) = \\sin(x)$\n",
    "\n",
    "Find value of all the above functions at $x = 2$.\n",
    "\n",
    "2. Let $f(x) = 3x - 1$ and $g(x) = \\sqrt{x}$. Find:\n",
    "   - $f(g(x))$\n",
    "   - $g(f(x))$\n",
    "   - $f(f(x))$\n",
    "   - $g(g(x))$\n",
    "\n",
    "and visualize functions in a single Geogebra notebook.\n",
    "\n",
    "3. Let $f(x) = e^x$ and $g(x) = \\ln(x)$. Check: $f(g(x))$ and $g(f(x))$. What do you notice?\n",
    "\n",
    "4. We have function $f=\\{(1,7), (2,9), (3,11)\\}$. Give inverse function $f^{-1}$.\n",
    "\n",
    "5. We have function $f=\\{(1,7), (2,7), (3,11)\\}$. Give inverse function $f^{-1}$.\n",
    "\n",
    "6. We have function $f(x)= x-1$. Give inverse function $f^{-1}$. Show both functions on the same Geogebra notebook."
   ]
  },
  {
   "cell_type": "markdown",
   "metadata": {},
   "source": [
    "<h2> SOLUTIONS </h2>\n",
    "<hr>\n",
    "\n",
    "# Solution 1\n",
    "\n",
    "[![Solution 1 with GeoGebra](https://i.postimg.cc/cJprSzXF/1.png)](https://postimg.cc/gwKYyg9h)\n",
    "\n",
    "# Solution 2\n",
    "\n",
    "[![Solution 2 with GeoGebra](https://i.postimg.cc/PrXP4G04/2.png)](https://postimg.cc/fkPzzPzt)\n",
    "\n",
    "# Solution 3\n",
    "To check the compositions $f(g(x))$ and $g(f(x))$ for the functions $f(x) = e^x$ and $g(x) = \\ln(x)$, follow these steps:\n",
    "\n",
    "1. **Compute \\( f(g(x)) \\):**\n",
    "   $$\n",
    "   f(g(x)) = f(\\ln(x)) = e^{\\ln(x)}\n",
    "   $$\n",
    "   Since $e^{\\ln(x)} = x$ (because the exponential function and the natural logarithm are inverse functions), we have:\n",
    "   $$\n",
    "   f(g(x)) = x\n",
    "   $$\n",
    "\n",
    "2. **Compute \\( g(f(x)) \\):**\n",
    "   $$\n",
    "   g(f(x)) = g(e^x) = \\ln(e^x)\n",
    "   $$\n",
    "   Similarly, $\\ln(e^x) = x$ (again, because they are inverse functions), so:\n",
    "   $$\n",
    "   g(f(x)) = x\n",
    "   $$\n",
    "\n",
    "**Observation:**\n",
    "Both compositions $f(g(x))$ and $g(f(x))$ simplify to $x$. This demonstrates that $f(x) = e^x$ and $g(x) = \\ln(x)$ are **inverse functions** of each other.\n",
    "\n",
    "$$\n",
    "\\boxed{f(g(x)) = g(f(x)) = x}\n",
    "$$\n",
    "\n",
    "\n",
    "# Solution 4\n",
    "\n",
    "**Solution:**  \n",
    "To find the inverse function $f^{-1}$, reverse the order of elements in each pair of $f$. \n",
    "\n",
    "Given:  \n",
    "$$\n",
    "f = \\{(1,7), \\ (2,9), \\ (3,11)\\}\n",
    "$$\n",
    "\n",
    "Reverse each pair \\((x, y)\\) to \\((y, x)\\):  \n",
    "$$\n",
    "(1,7) \\rightarrow (7,1), \\quad (2,9) \\rightarrow (9,2), \\quad (3,11) \\rightarrow (11,3)\n",
    "$$\n",
    "\n",
    "**Answer:**  \n",
    "$$\n",
    "f^{-1} = \\{(7,1), \\ (9,2), \\ (11,3)\\}\n",
    "$$\n",
    "\n",
    "# Solution 5\n",
    "\n",
    "**Solution:**  \n",
    "To find the inverse relation $f^{-1}$, reverse the order of elements in each pair of $f$.\n",
    "\n",
    "Given:  \n",
    "$$\n",
    "f = \\{(1,7), \\ (2,7), \\ (3,11)\\}\n",
    "$$\n",
    "\n",
    "Reverse each pair \\((x, y)\\) to \\((y, x)\\):  \n",
    "$$\n",
    "(1,7) \\rightarrow (7,1), \\quad (2,7) \\rightarrow (7,2), \\quad (3,11) \\rightarrow (11,3)\n",
    "$$\n",
    "\n",
    "**Important Note:**  \n",
    "The original function \\( f \\) is **not injective** (one-to-one) because both \\( x=1 \\) and \\( x=2 \\) map to \\( y=7 \\). As a result, the inverse \\( f^{-1} \\) is **not a valid function** (it fails the vertical line test). It is instead a *relation* with multiple outputs for the same input.\n",
    "\n",
    "**Answer (as a relation):**  \n",
    "$$\n",
    "f^{-1} = \\{(7,1), \\ (7,2), \\ (11,3)\\}\n",
    "$$\n",
    "\n",
    "\n",
    "# Solution 6\n",
    "\n",
    "**Answer**\n",
    "\n",
    "The inverse function of $f(x) = x - 1$ is $f^{-1}(x) = x + 1$.\n",
    "\n",
    "**Functions**:  \n",
    "- **Original function**:  \n",
    "  $$ f(x) = x - 1 $$  \n",
    "- **Inverse function**:  \n",
    "  $$ f^{-1}(x) = x + 1 $$  \n",
    "\n",
    " \n",
    "\n",
    "**Key Observations**:  \n",
    "- Both lines have a slope of \\( 1 \\).  \n",
    "- $f(x)$ has a $y$-intercept at $-1$, while $f^{-1}(x)$ has a $y$-intercept at $1$. \n",
    "- They are reflections of each other over \\( y = x \\).  \n",
    "\n",
    "[![Solution 6 with GeoGebra](https://i.postimg.cc/ZYghYnd2/7.png)](https://postimg.cc/RqcYXMGL)\n",
    "\n"
   ]
  }
 ],
 "metadata": {
  "language_info": {
   "name": "python"
  }
 },
 "nbformat": 4,
 "nbformat_minor": 2
}
