{
 "cells": [
  {
   "cell_type": "markdown",
   "metadata": {},
   "source": [
    "## 23. Taylor Series\n",
    "\n",
    "1. Find the Taylor series and visualize obtained functions in Geogebra:\n",
    "   - $f(x) = \\cos(x)$ around $x = 0$ up to the 4th degree.\n",
    "   - $h(x) = 1/(1-x)$ around $x = 0$ up to the 4rd degree.\n",
    "   - $g(x) = \\sin(x)$ around $x = \\pi$ up to the 4rd degree.\n",
    "\n",
    "2. Find a tangent line $y = f'(x_0) (x-x_0) + f(x_0)$ to the function $f(x) = e^{\\sin(x)}$ at $x_0 = \\pi$. Hints for Geogebra visualization: define f(x), include slider s, define y = f'(s) (x-s) + f(s), and include point P(s, f(s))."
   ]
  },
  {
   "cell_type": "markdown",
   "metadata": {},
   "source": [
    "<h2> SOLUTIONS </h2>\n",
    "<hr>\n",
    "\n",
    "# Solution 1\n",
    "\n",
    "**1. Taylor Series for $f(x) = \\cos(x)$ around $x = 0$ up to the 4th degree**\n",
    "\n",
    "The Taylor series for a function $f(x)$ around $x = a$ is given by:\n",
    "\n",
    "$f(x) = f(a) + f'(a)(x-a) + \\frac{f''(a)}{2!}(x-a)^2 + \\frac{f'''(a)}{3!}(x-a)^3 + \\frac{f''''(a)}{4!}(x-a)^4 + \\cdots$\n",
    "\n",
    "For $f(x) = \\cos(x)$ around $x = 0$:\n",
    "\n",
    "* $f(x) = \\cos(x)$, so $f(0) = 1$\n",
    "* $f'(x) = -\\sin(x)$, so $f'(0) = 0$\n",
    "* $f''(x) = -\\cos(x)$, so $f''(0) = -1$\n",
    "* $f'''(x) = \\sin(x)$, so $f'''(0) = 0$\n",
    "* $f''''(x) = \\cos(x)$, so $f''''(0) = 1$\n",
    "\n",
    "Substituting into the Taylor series formula:\n",
    "\n",
    "$\\cos(x) \\approx 1 + 0\\cdot x + \\frac{-1}{2!}x^2 + \\frac{0}{3!}x^3 + \\frac{1}{4!}x^4$\n",
    "\n",
    "Simplifying:\n",
    "\n",
    "$\\cos(x) \\approx 1 - \\frac{x^2}{2} + \\frac{x^4}{24}$\n",
    "\n",
    "\n",
    "**2. Taylor Series for $h(x) = \\frac{1}{1-x}$ around $x = 0$ up to the 4th degree**\n",
    "\n",
    "For $h(x) = \\frac{1}{1-x}$, the derivatives are:\n",
    "\n",
    "* $h(x) = \\frac{1}{1-x}$, so $h(0) = 1$\n",
    "* $h'(x) = \\frac{1}{(1-x)^2}$, so $h'(0) = 1$\n",
    "* $h''(x) = \\frac{2}{(1-x)^3}$, so $h''(0) = 2$\n",
    "* $h'''(x) = \\frac{6}{(1-x)^4}$, so $h'''(0) = 6$\n",
    "* $h''''(x) = \\frac{24}{(1-x)^5}$, so $h''''(0) = 24$\n",
    "\n",
    "Substituting into the Taylor series formula:\n",
    "\n",
    "$h(x) \\approx h(0) + h'(0)x + \\frac{h''(0)}{2!}x^2 + \\frac{h'''(0)}{3!}x^3 + \\frac{h''''(0)}{4!}x^4$\n",
    "\n",
    "$h(x) \\approx 1 + x + \\frac{2}{2!}x^2 + \\frac{6}{3!}x^3 + \\frac{24}{4!}x^4$\n",
    "\n",
    "Simplifying:\n",
    "\n",
    "$h(x) \\approx 1 + x + x^2 + x^3 + x^4$\n",
    "\n",
    "\n",
    "**3. Taylor Series for $g(x) = \\sin(x)$ around $x = \\pi$ up to the 4th degree**\n",
    "\n",
    "For $g(x) = \\sin(x)$, the derivatives are:\n",
    "\n",
    "* $g(x) = \\sin(x)$, so $g(\\pi) = 0$\n",
    "* $g'(x) = \\cos(x)$, so $g'(\\pi) = -1$\n",
    "* $g''(x) = -\\sin(x)$, so $g''(\\pi) = 0$\n",
    "* $g'''(x) = -\\cos(x)$, so $g'''(\\pi) = 1$\n",
    "* $g''''(x) = \\sin(x)$, so $g''''(π) = 0$\n",
    "\n",
    "Substituting into the Taylor series formula:\n",
    "\n",
    "$g(x) \\approx g(\\pi) + g'(\\pi)(x-\\pi) + \\frac{g''(\\pi)}{2!}(x-\\pi)^2 + \\frac{g'''(\\pi)}{3!}(x-\\pi)^3 + \\frac{g''''(π)}{4!}(x-\\pi)^4$\n",
    "\n",
    "$g(x) \\approx 0 + (-1)(x-\\pi) + \\frac{0}{2!}(x-\\pi)^2 + \\frac{1}{3!}(x-\\pi)^3 + \\frac{0}{4!}(x-\\pi)^4$\n",
    "\n",
    "Simplifying:\n",
    "\n",
    "$g(x) \\approx -(x-\\pi) + \\frac{(x-\\pi)^3}{6}$\n",
    "\n",
    "[![Solution 1 with GeoGebra](https://i.postimg.cc/5y3PpGNQ/1-1.png)](https://postimg.cc/LgJB8xPm)\n",
    "\n",
    "# Solution 2\n",
    "\n",
    "**Finding the Tangent Line**\n",
    "\n",
    "**Step 1: Compute $f(x_0)$**\n",
    "\n",
    "Evaluate $f(x)$ at $x_0 = \\pi$:\n",
    "\n",
    "$f(\\pi) = e^{\\sin(\\pi)} = e^0 = 1$\n",
    "\n",
    "**Step 2: Compute the derivative $f'(x)$**\n",
    "\n",
    "Use the chain rule to differentiate $f(x) = e^{\\sin(x)}$:\n",
    "\n",
    "$f'(x) = \\frac{d}{dx}(e^{\\sin(x)}) = e^{\\sin(x)} \\cdot \\cos(x)$\n",
    "\n",
    "**Step 3: Evaluate $f'(x_0)$**\n",
    "\n",
    "Evaluate $f'(x)$ at $x_0 = \\pi$:\n",
    "\n",
    "$f'(\\pi) = e^{\\sin(\\pi)} \\cdot \\cos(\\pi) = e^0 \\cdot (-1) = -1$\n",
    "\n",
    "**Step 4: Write the tangent line equation**\n",
    "\n",
    "Using the point-slope form of a line, the tangent line at $x_0 = \\pi$ is:\n",
    "\n",
    "$y = f'(\\pi)(x - \\pi) + f(\\pi)$\n",
    "\n",
    "Substitute $f'(\\pi) = -1$ and $f(\\pi) = 1$:\n",
    "\n",
    "$y = -1 \\cdot (x - \\pi) + 1$\n",
    "\n",
    "Simplify:\n",
    "\n",
    "$y = -x + \\pi + 1$\n",
    "\n",
    "**Final Answer:**\n",
    "\n",
    "The tangent line to $f(x) = e^{\\sin(x)}$ at $x_0 = \\pi$ is:\n",
    "\n",
    "$y = -x + \\pi + 1$\n",
    "\n",
    "[![Solution 2 with GeoGebra](https://i.postimg.cc/Kcp3Prts/2-2.png)](https://postimg.cc/MXRGxBPy)"
   ]
  }
 ],
 "metadata": {
  "language_info": {
   "name": "python"
  }
 },
 "nbformat": 4,
 "nbformat_minor": 2
}
