{
 "cells": [
  {
   "cell_type": "markdown",
   "metadata": {},
   "source": [
    "## 25. Differential Equations\n",
    "\n",
    "1. Solve the following first-order ordinary differential equations:\n",
    "   - $y'(x)= y(x)$\n",
    "   - $y'(x) = \\frac{1}{2y(x)}$\n",
    "  \n",
    "3. Solve the first-order ordinary differential equations using the method of separation of variables for $x$ and $y=y(x)$:\n",
    "\n",
    "   - $\\frac{dy}{dx} = \\frac{x}{y}$\n",
    "   - $\\frac{dy}{dx} = \\frac{y}{x}$\n",
    "   - $\\frac{dy}{dx} = xy$\n",
    "\n",
    "4. Solve the second-order ordinary differential equations:\n",
    "\n",
    "   * $y''(x) + y'(x) = 0$, with boundary conditions $y(0) = 2$ and $y'(0) = -1$\n",
    "\n",
    "   * $y''(x) - y(x)= 0$, with boundary conditions $y(0) = 2$ and $y'(0) = 0$\n",
    "\n",
    "   * $\\frac{d^2 y(x)}{dx^2} = -\\omega^2 y(x)$.\n",
    "  \n",
    "5. Check if the function $\\psi(t, x) = A \\cos(\\omega t + kx)$ is a solution of the second-order partial differential equation (the so-called \"wave equation\"), where $v = \\frac{\\omega}{k} = \\frac{2\\pi / T}{2\\pi / \\lambda}$:\n",
    "\n",
    "$$\n",
    "\\frac{\\partial^2 \\psi(t, x)}{\\partial t^2} - v^2 \\frac{\\partial^2 \\psi(t, x)}{\\partial x^2} = 0.\n",
    "$$"
   ]
  },
  {
   "cell_type": "markdown",
   "metadata": {},
   "source": [
    "<h2> SOLUTIONS </h2>\n",
    "<hr>\n",
    "\n",
    "# Solution 1\n",
    "\n",
    "**Solve $y'(x) = y(x)$:**\n",
    "\n",
    "This is a separable differential equation. We can rewrite it as:\n",
    "\n",
    "$\\frac{dy}{dx} = y$\n",
    "\n",
    "Separate the variables:\n",
    "\n",
    "$\\frac{dy}{y} = dx$\n",
    "\n",
    "Integrate both sides:\n",
    "\n",
    "$\\int \\frac{dy}{y} = \\int dx$\n",
    "\n",
    "$\\ln|y| = x + C$\n",
    "\n",
    "Exponentiate both sides to solve for $y$:\n",
    "\n",
    "$y(x) = e^{x+C} = e^C e^x$\n",
    "\n",
    "Let $C_1 = e^C$ (where $C_1 > 0$):\n",
    "\n",
    "$y(x) = C_1 e^x$\n",
    "\n",
    "Final Answer:\n",
    "\n",
    "$y(x) = C_1 e^x$\n",
    "\n",
    "---\n",
    "\n",
    "**Solve $y'(x) = \\frac{1}{2}y(x)$:**\n",
    "\n",
    "This is also a separable differential equation. Rewrite it as:\n",
    "\n",
    "$\\frac{dy}{dx} = \\frac{1}{2}y$\n",
    "\n",
    "Separate the variables:\n",
    "\n",
    "$\\frac{2}{y} dy = dx$\n",
    "\n",
    "Integrate both sides:\n",
    "\n",
    "$\\int \\frac{2}{y} dy = \\int dx$\n",
    "\n",
    "$2\\ln|y| = x + C$\n",
    "\n",
    "$\\ln|y|^2 = x+C$\n",
    "\n",
    "$|y|^2 = e^{x+C} = e^C e^x$\n",
    "\n",
    "$y^2 = Ae^x$ where $A = e^C > 0$\n",
    "\n",
    "\n",
    "Solve for $y$:\n",
    "\n",
    "$y(x) = \\pm \\sqrt{Ae^x} = \\pm \\sqrt{A} e^{x/2}$\n",
    "\n",
    "Let $C_1 = \\pm\\sqrt{A}$, then\n",
    "\n",
    "$y(x) = C_1 e^{x/2}$ where $C_1 \\ne 0$.\n",
    "\n",
    "If $y=0$, then $y'=0$ and $y = \\frac{1}{2}y$ is satisfied.  So $y(x) = 0$ is also a solution.\n",
    "\n",
    "Final Answer:\n",
    "\n",
    "$y(x) = C_1 e^{x/2}$ where $C_1$ is a real number.\n",
    "\n",
    "# Solution 2\n",
    "\n",
    "1. $\\frac{dy}{dx} = \\frac{y}{x}$\n",
    "\n",
    "Step 1: Separate the variables $x$ and $y$:\n",
    "\n",
    "$y \\, dy = x \\, dx$\n",
    "\n",
    "Step 2: Integrate both sides:\n",
    "\n",
    "$\\int y \\, dy = \\int x \\, dx$\n",
    "\n",
    "$\\frac{y^2}{2} = \\frac{x^2}{2} + C$\n",
    "\n",
    "where $C$ is the constant of integration.\n",
    "\n",
    "Step 3: Solve for $y$:\n",
    "\n",
    "$y^2 = x^2 + 2C$\n",
    "\n",
    "$y = \\pm \\sqrt{x^2 + 2C}$\n",
    "\n",
    "Final Solution:\n",
    "\n",
    "$y = \\pm \\sqrt{x^2 + C'}$\n",
    "\n",
    "where $C' = 2C$ is a new constant.\n",
    "\n",
    "---\n",
    "\n",
    "2. $\\frac{dy}{dx} = \\frac{x}{y}$\n",
    "\n",
    "Step 1: Separate the variables $x$ and $y$:\n",
    "\n",
    "$\\frac{dy}{y} = \\frac{dx}{x}$\n",
    "\n",
    "Step 2: Integrate both sides:\n",
    "\n",
    "$\\int \\frac{dy}{y} = \\int \\frac{dx}{x}$\n",
    "\n",
    "$\\ln|y| = \\ln|x| + C$\n",
    "\n",
    "where $C$ is the constant of integration.\n",
    "\n",
    "Step 3: Solve for $y$:\n",
    "\n",
    "$|y| = e^{\\ln|x| + C} = e^{\\ln|x|} \\cdot e^C = |x| \\cdot e^C$\n",
    "\n",
    "$y = \\pm e^C x$\n",
    "\n",
    "Final Solution:\n",
    "\n",
    "$y = C'x$\n",
    "\n",
    "where $C' = \\pm e^C$ is a new constant.\n",
    "\n",
    "---\n",
    "\n",
    "3. $\\frac{dy}{dx} = xy$\n",
    "\n",
    "Step 1: Separate the variables $x$ and $y$:\n",
    "\n",
    "$\\frac{dy}{y} = x \\, dx$\n",
    "\n",
    "Step 2: Integrate both sides:\n",
    "\n",
    "$\\int \\frac{dy}{y} = \\int x \\, dx$\n",
    "\n",
    "$\\ln|y| = \\frac{x^2}{2} + C$\n",
    "\n",
    "where $C$ is the constant of integration.\n",
    "\n",
    "Step 3: Solve for $y$:\n",
    "\n",
    "$|y| = e^{\\frac{x^2}{2} + C} = e^{\\frac{x^2}{2}} \\cdot e^C$\n",
    "\n",
    "$y = \\pm e^C e^{\\frac{x^2}{2}}$\n",
    "\n",
    "Final Solution:\n",
    "\n",
    "$y = C' e^{\\frac{x^2}{2}}$\n",
    "\n",
    "where $C' = \\pm e^C$ is a new constant.\n",
    "\n",
    "---\n",
    "\n",
    "Summary of Solutions:\n",
    "\n",
    "$\\frac{dy}{dx} = \\frac{y}{x} \\rightarrow y = \\pm \\sqrt{x^2 + C'}$\n",
    "\n",
    "$\\frac{dy}{dx} = \\frac{x}{y} \\rightarrow y = C'x$\n",
    "\n",
    "$\\frac{dy}{dx} = xy \\rightarrow y = C' e^{\\frac{x^2}{2}}$\n",
    "\n",
    "# Solution 3\n",
    "\n",
    "**Problem 1:** $y''(x) + y'(x) = 0$ with boundary conditions $y(0) = 2$ and $y'(0) = -1$\n",
    "\n",
    "**Step 1:** Find the characteristic equation.\n",
    "\n",
    "The differential equation is:\n",
    "\n",
    "$y''(x) + y'(x) = 0$\n",
    "\n",
    "Assume a solution of the form $y(x) = e^{rx}$. Substituting into the equation gives:\n",
    "\n",
    "$r^2e^{rx} + re^{rx} = 0 \\implies r^2 + r = 0$\n",
    "\n",
    "The characteristic equation is:\n",
    "\n",
    "$r^2 + r = 0$\n",
    "\n",
    "**Step 2:** Solve the characteristic equation.\n",
    "\n",
    "$r(r+1) = 0 \\implies r = 0$ or $r = -1$\n",
    "\n",
    "**Step 3:** Write the general solution.\n",
    "\n",
    "The general solution is:\n",
    "\n",
    "$y(x) = C_1e^{0x} + C_2e^{-x} = C_1 + C_2e^{-x}$\n",
    "\n",
    "**Step 4:** Apply the boundary conditions to find $C_1$ and $C_2$.\n",
    "\n",
    "$y(0) = 2$:\n",
    "\n",
    "$C_1 + C_2e^0 = C_1 + C_2 = 2$\n",
    "\n",
    "$y'(x) = -C_2e^{-x}$, so $y'(0) = -1$:\n",
    "\n",
    "$-C_2e^0 = -C_2 = -1 \\implies C_2 = 1$\n",
    "\n",
    "Substitute $C_2 = 1$ into the first equation:\n",
    "\n",
    "$C_1 + 1 = 2 \\implies C_1 = 1$\n",
    "\n",
    "**Step 5:** Write the final solution.\n",
    "\n",
    "$y(x) = 1 + e^{-x}$\n",
    "\n",
    "---\n",
    "\n",
    "**Problem 2:** $y''(x) - y(x) = 0$ with boundary conditions $y(0) = 2$ and $y'(0) = 0$\n",
    "\n",
    "**Step 1:** Find the characteristic equation.\n",
    "\n",
    "The differential equation is:\n",
    "\n",
    "$y''(x) - y(x) = 0$\n",
    "\n",
    "Assume a solution of the form $y(x) = e^{rx}$. Substituting into the equation gives:\n",
    "\n",
    "$r^2e^{rx} - e^{rx} = 0 \\implies r^2 - 1 = 0$\n",
    "\n",
    "The characteristic equation is:\n",
    "\n",
    "$r^2 - 1 = 0$\n",
    "\n",
    "**Step 2:** Solve the characteristic equation.\n",
    "\n",
    "$r^2 - 1 = 0 \\implies r = \\pm 1$\n",
    "\n",
    "**Step 3:** Write the general solution.\n",
    "\n",
    "The general solution is:\n",
    "\n",
    "$y(x) = C_1e^x + C_2e^{-x}$\n",
    "\n",
    "**Step 4:** Apply the boundary conditions to find $C_1$ and $C_2$.\n",
    "\n",
    "$y(0) = 2$:\n",
    "\n",
    "$C_1e^0 + C_2e^0 = C_1 + C_2 = 2$\n",
    "\n",
    "$y'(x) = C_1e^x - C_2e^{-x}$, so $y'(0) = 0$:\n",
    "\n",
    "$C_1e^0 - C_2e^0 = C_1 - C_2 = 0 \\implies C_1 = C_2$\n",
    "\n",
    "Substitute $C_1 = C_2$ into the first equation:\n",
    "\n",
    "$C_1 + C_1 = 2 \\implies 2C_1 = 2 \\implies C_1 = 1$\n",
    "\n",
    "Thus, $C_2 = 1$.\n",
    "\n",
    "**Step 5:** Write the final solution.\n",
    "\n",
    "$y(x) = e^x + e^{-x}$  or $y(x) = 2\\cosh(x)$\n",
    "\n",
    "---\n",
    "\n",
    "**Problem 3:** $\\frac{d^2y(x)}{dx^2} = -\\omega^2 y(x)$\n",
    "\n",
    "**Step 1:** Rewrite the differential equation.\n",
    "\n",
    "The differential equation is:\n",
    "\n",
    "$\\frac{d^2y(x)}{dx^2} + \\omega^2 y(x) = 0$\n",
    "\n",
    "**Step 2:** Find the characteristic equation.\n",
    "\n",
    "Assume a solution of the form $y(x) = e^{rx}$. Substituting into the equation gives:\n",
    "\n",
    "$r^2e^{rx} + \\omega^2e^{rx} = 0 \\implies r^2 + \\omega^2 = 0$\n",
    "\n",
    "The characteristic equation is:\n",
    "\n",
    "$r^2 + \\omega^2 = 0$\n",
    "\n",
    "**Step 3:** Solve the characteristic equation.\n",
    "\n",
    "$r^2 + \\omega^2 = 0 \\implies r = \\pm i\\omega$\n",
    "\n",
    "**Step 4:** Write the general solution.\n",
    "\n",
    "The general solution is:\n",
    "\n",
    "$y(x) = C_1\\cos(\\omega x) + C_2\\sin(\\omega x)$\n",
    "\n",
    "**Step 5:** Apply boundary conditions (if provided).\n",
    "\n",
    "No boundary conditions are given, so the general solution is:\n",
    "\n",
    "$y(x) = C_1\\cos(\\omega x) + C_2\\sin(\\omega x)$\n",
    "\n",
    "# Solution 4\n",
    "\n",
    "To determine if the function $\\psi(t,x) = A\\cos(\\omega t + kx)$ is a solution to the wave equation:\n",
    "\n",
    "$$\\frac{\\partial^2\\psi(t,x)}{\\partial t^2} - v^2\\frac{\\partial^2\\psi(t,x)}{\\partial x^2} = 0,$$\n",
    "\n",
    "we need to compute the second partial derivatives of $\\psi(t,x)$ with respect to $t$ and $x$, and then substitute them into the wave equation.\n",
    "\n",
    "**Step 1: Compute $\\frac{\\partial^2\\psi(t,x)}{\\partial t^2}$**\n",
    "\n",
    "First, compute the first partial derivative of $\\psi(t,x)$ with respect to $t$:\n",
    "\n",
    "$$\\frac{\\partial\\psi(t,x)}{\\partial t} = -A\\omega\\sin(\\omega t + kx).$$\n",
    "\n",
    "Next, compute the second partial derivative with respect to $t$:\n",
    "\n",
    "$$\\frac{\\partial^2\\psi(t,x)}{\\partial t^2} = -A\\omega^2\\cos(\\omega t + kx).$$\n",
    "\n",
    "**Step 2: Compute $\\frac{\\partial^2\\psi(t,x)}{\\partial x^2}$**\n",
    "\n",
    "First, compute the first partial derivative of $\\psi(t,x)$ with respect to $x$:\n",
    "\n",
    "$$\\frac{\\partial\\psi(t,x)}{\\partial x} = -Ak\\sin(\\omega t + kx).$$\n",
    "\n",
    "Next, compute the second partial derivative with respect to $x$:\n",
    "\n",
    "$$\\frac{\\partial^2\\psi(t,x)}{\\partial x^2} = -Ak^2\\cos(\\omega t + kx).$$\n",
    "\n",
    "**Step 3: Substitute into the wave equation**\n",
    "\n",
    "Substitute the second derivatives into the wave equation:\n",
    "\n",
    "$$\\frac{\\partial^2\\psi(t,x)}{\\partial t^2} - v^2\\frac{\\partial^2\\psi(t,x)}{\\partial x^2} = 0.$$\n",
    "\n",
    "Substituting the expressions we found:\n",
    "\n",
    "$$-A\\omega^2\\cos(\\omega t + kx) - v^2(-Ak^2\\cos(\\omega t + kx)) = 0.$$\n",
    "\n",
    "Simplify the equation:\n",
    "\n",
    "$$-A\\omega^2\\cos(\\omega t + kx) + Av^2k^2\\cos(\\omega t + kx) = 0.$$\n",
    "\n",
    "Factor out $A\\cos(\\omega t + kx)$:\n",
    "\n",
    "$$A\\cos(\\omega t + kx)(-\\omega^2 + v^2k^2) = 0.$$\n",
    "\n",
    "For this equation to hold for all $t$ and $x$, the coefficient must be zero:\n",
    "\n",
    "$$-\\omega^2 + v^2k^2 = 0.$$\n",
    "\n",
    "This implies:\n",
    "\n",
    "$$v^2 = \\frac{\\omega^2}{k^2}.$$\n",
    "\n",
    "Given that $v = \\frac{\\omega}{k}$, this condition is satisfied:\n",
    "\n",
    "$$v^2 = \\left(\\frac{\\omega}{k}\\right)^2 = \\frac{\\omega^2}{k^2}.$$\n",
    "\n",
    "**Conclusion**\n",
    "\n",
    "Since the condition $v^2 = \\frac{\\omega^2}{k^2}$ holds true, the function $\\psi(t,x) = A\\cos(\\omega t + kx)$ is indeed a solution to the wave equation.\n",
    "\n",
    "Yes, $\\psi(t,x) = A\\cos(\\omega t + kx)$ is a solution to the wave equation."
   ]
  }
 ],
 "metadata": {
  "language_info": {
   "name": "python"
  }
 },
 "nbformat": 4,
 "nbformat_minor": 2
}
